Changed so much... So much to go...

WebAssembly/Wasm.thy
@@ -90,7 +90,7 @@ and       s_typing :: "[s_context, (t list) option, nat, v list, e list, t list]
   (* callcl *)
 | "\<lbrakk>cl_typing \<S> cl tf\<rbrakk> \<Longrightarrow> \<S>\<bullet>\<C>  \<turnstile> [Callcl cl] : tf"
   (* tailcallcl *)
-| "\<lbrakk>cl_typing \<S> cl tf\<rbrakk> \<Longrightarrow> \<S>\<bullet>\<C>  \<turnstile> [TailCallcl cl] : tf"
+| "\<lbrakk>cl_typing \<S> cl (t1s _> t2s)\<rbrakk> \<Longrightarrow> \<S>\<bullet>\<C>  \<turnstile> [TailCallcl cl] : (t3s @ t1s _> t4s)"
   (* label *)
 | "\<lbrakk>\<S>\<bullet>\<C> \<turnstile> e0s : (ts _> t2s); \<S>\<bullet>\<C>\<lparr>label := ([ts] @ (label \<C>))\<rparr> \<turnstile> es : ([] _> t2s); length ts = n\<rbrakk> \<Longrightarrow> \<S>\<bullet>\<C> \<turnstile> [Label n e0s es] : ([] _> t2s)"
 (* section: s_typing *)
@@ -209,10 +209,9 @@ inductive reduce :: "[s, v list, e list, nat, s, v list, e list] \<Rightarrow> b
 | return_call_indirect_None:"\<lbrakk>(stab s i (nat_of_int c) = Some cl \<and> stypes s i j \<noteq> cl_type cl) \<or> stab s i (nat_of_int c) = None\<rbrakk> \<Longrightarrow> \<lparr>s;vs;[$C (ConstInt32 c), $(ReturnCall_indirect j)]\<rparr> \<leadsto>_i \<lparr>s;vs;[Trap]\<rparr>"
   \<comment> \<open>\<open>call\<close>\<close>
 | callcl_native:"\<lbrakk>cl = Func_native j (t1s _> t2s) ts es; ves = ($$* vcs); length vcs = n; length ts = k; length t1s = n; length t2s = m; (n_zeros ts = zs) \<rbrakk> \<Longrightarrow> \<lparr>s;vs;ves @ [Callcl cl]\<rparr> \<leadsto>_i \<lparr>s;vs;[Local m j (vcs@zs) [$(Block ([] _> t2s) es)]]\<rparr>"
-| tail_callcl_native:"\<lbrakk>cl = Func_native j (t1s _> t2s) ts bes; ves = ($$* vcs); length vcs = n; length t1s = n; length t2s = m; Lfilled k lholed (ves @ [TailCallcl cl]) es\<rbrakk> \<Longrightarrow> \<lparr>s;vs;ves @ [TailCallcl cl]\<rparr> \<leadsto>_i \<lparr>s;vs;ves@[Callcl cl]\<rparr>"
 | callcl_host_Some:"\<lbrakk>cl = Func_host (t1s _> t2s) f; ves = ($$* vcs); length vcs = n; length t1s = n; length t2s = m; host_apply s (t1s _> t2s) f vcs hs = Some (s', vcs')\<rbrakk> \<Longrightarrow> \<lparr>s;vs;ves @ [Callcl cl]\<rparr> \<leadsto>_i \<lparr>s';vs;($$* vcs')\<rparr>"
 | callcl_host_None:"\<lbrakk>cl = Func_host (t1s _> t2s) f; ves = ($$* vcs); length vcs = n; length t1s = n; length t2s = m\<rbrakk> \<Longrightarrow> \<lparr>s;vs;ves @ [Callcl cl]\<rparr> \<leadsto>_i \<lparr>s;vs;[Trap]\<rparr>"
-| tail_callcl_host:"\<lbrakk>cl = Func_host (t1s _> t2s) f\<rbrakk> \<Longrightarrow> \<lparr>s;vs;ves @ [TailCallcl cl]\<rparr> \<leadsto>_i \<lparr>s;vs;[Trap]\<rparr>"
+| tail_callcl:"\<lbrakk>cl_type cl = (t1s _> t2s); const_list vcs; length vcs = n; length t1s = n; length t2s = m; Lfilled j lholed (vcs @ [TailCallcl cl]) es\<rbrakk> \<Longrightarrow> \<lparr>s;vs;[Local n k vls es]\<rparr> \<leadsto>_i \<lparr>s;vs;vcs@[Callcl cl]\<rparr>"
   \<comment> \<open>\<open>get_local\<close>\<close>
 | get_local:"\<lbrakk>length vi = j\<rbrakk> \<Longrightarrow> \<lparr>s;(vi @ [v] @ vs);[$(Get_local j)]\<rparr> \<leadsto>_i \<lparr>s;(vi @ [v] @ vs);[$(C v)]\<rparr>"
   \<comment> \<open>\<open>set_local\<close>\<close>
